A VCache.fsti that type-checks

experiments/Veritas.VCache.fsti
@@ -1,6 +1,9 @@
 module Veritas.VCache
 
-open VerifierTraits
+module B = LowStar.Buffer
+module HS = FStar.HyperStack
+
+open FStar.HyperStack.ST
 
 /// Based on veritas/verifier/vcache.h
 ///
@@ -30,20 +33,21 @@ open VerifierTraits
 ///
 /// Note: this is a value which greatly simplifies things in Low*.
 type addr = {
-  a0:uint_64;
-  a1:uint_64;
-  a2:uint_64;
-  a3:uint_64
+  a0:UInt64.t;
+  a1:UInt64.t;
+  a2:UInt64.t;
+  a3:UInt64.t
 }
 
 /// From merkle.h
 /// Merkle address identifies a location in the sparse merkle tree
 type merkle_addr = {
   path: addr;
-  depth: uint_16
+  depth: UInt16.t
 }
 
 /// From merkle_vcell.h
+noeq
 type merkle_leaf = {
   addr: merkle_addr;   //32 bytes
   data_vcell: B.pointer VCell.t
@@ -60,28 +64,25 @@ type merkle_internal =
    left: hash_value;    // Typically, say, 32 bytes as a pair of UInt128s
    right: hash_value;
    dpath: addr & addr; // Not yet sure exactly what these additional fields represent
-   depth: uint32;
-   ddepth: uint16 & uint16
+   depth: UInt32.t;
+   ddepth: UInt16.t & UInt16.t
 }
 
-/// From vcache.h
-/// CachePolicy is an enum in C++. We encode it ...
-///
-/// JP: we voted against ``type cache_policy = Merkle | Blum | BlumHash``. Why?
-/// (The constants would be 1, 2, 3 instead of 1, 2, 4 but not a big deal?). It
-/// would also give use pattern-matches.
-let merkle = 0x01ul
-let blum = 0x02ul
-let blum_hash = 0x04ul
-let cache_policy = u:uint8_t{ u = 0x01 \/ u = 0x02 \/ u=0x04 }
+/// CachePolicy, from veritas/common/common.h
+type cache_policy =
+  | Merkle
+  | Blum
+  | BlumHash
 
 /// A slot in the cache stores either a leaf or an internal node
+noeq
 type slot =
   | MerkleLeaf  of merkle_leaf
   | MerkleInternal of merkle_internal
 
 
 /// An entry is a slot paired with the metadata for use by the cache
+noeq
 type entry = {
   slot: slot; // this is the field that is an std::array<uint64, 20> in C++
   cp: cache_policy;
@@ -89,71 +90,84 @@ type entry = {
   touched: bool;
 }
 
+let lbuffer a l =
+  b:B.buffer a { B.length b == l }
+
 /// The main type provided by vcache encapsulates a fixed array of
 /// cache entries.
 ///
+/// Note that the run-time representation does not depend on t (otherwise, a
+/// trick like https://github.com/FStarLang/kremlin/issues/183 would be needed).
+///
+/// TODO: hide this behind the abstraction once it's ready.
+noeq
 type t (tr: VerifierTraits.t) = {
-  entries:Buffer.lbuffer entry (UInt32.v tr.cache_size)
+  entries: lbuffer entry (UInt16.v tr.VerifierTraits.cache_size)
 }
 
 /// Stateful API
 /// ------------
+///
+/// In order to make sure you're not forgetting anything, it's always a good
+/// idea to refer to hacl-star/code/streaming/Hacl.Streaming.Interface and make
+/// sure you're implementing at least the stateful type class, which is the bare
+/// minimum for your clients to be able to do something with your code.
 
 /// We have some abstract invariants on caches, e.g., liveness properties etc.
-val cache_invariant (#v:Type) [| verifier_traits v |] (c: t v) : mem -> prop
+/// This also includes freeable, which we'll need to implement the free function.
+val invariant (#tr: VerifierTraits.t) (h: HS.mem) (cache: t tr): Type0
 
-/// We have to aim for a static footprint. Note that this is just about the
-/// array of entries, not the vcells pointed to by the entries themselves (to be
-/// discussed).
-val footprint: #v:Type -> [| verified_traits v |] -> t v -> B.loc
+/// We aim for a static footprint. Note that this is just about the array of
+/// entries, knowing that vcells are values means that we don't have to be more
+/// complicated than that.
+val footprint (#tr: VerifierTraits.t) (cache: t tr): GTot B.loc
 
-val frame_invariant: #v:Type -> [| verified_traits v |] -> l:B.loc -> h0:HS.mem -> h1:HS.mem -> c:t v -> Lemma
-  (requires (
-    B.modifies l h0 h1 /\
-    B.loc_disjoint l (footprint c) /\
-    cache_invariant c h0))
-  (ensures (
-    cache_invariant c h1))
+val invariant_loc_in_footprint: #tr:VerifierTraits.t -> h:HS.mem -> cache:t tr -> Lemma
+    (requires (invariant h cache))
+    (ensures (B.loc_in (footprint cache) h))
+    [ SMTPat (invariant h cache) ]
 
 /// For spec purposes, a cache is a sequence of entries
-val entries (#v:_) [|verifier_traits v] (c:t v) (m:mem{cache_invariant c m})
-  : GTot (seq entry)
+val entries (#tr: VerifierTraits.t) (h: HS.mem) (cache: t tr):
+  GTot (Seq.lseq entry (UInt16.v (tr.VerifierTraits.cache_size)))
+
+val frame_invariant: #tr:VerifierTraits.t -> l:B.loc -> cache:t tr -> h0:HS.mem -> h1:HS.mem -> Lemma
+    (requires (
+      invariant h0 cache /\
+      B.loc_disjoint l (footprint cache) /\
+      B.modifies l h0 h1))
+    (ensures (
+      invariant h1 cache /\
+      entries h0 cache == entries h1 cache /\
+      footprint cache == footprint cache))
+    [ SMTPat (invariant h1 cache); SMTPat (B.modifies l h0 h1) ]
 
 /// Cache entries are indexed by u16 values
-let vcache_idx = uint_16
+let vcache_idx = UInt16.t
 
 /// The C++ API allows looking up cache entries and returns them by reference.
-/// These references are the read and mutated by client code in vmem_vops.h etc.
+/// These references are then read and mutated by client code in vmem_vops.h etc.
 ///
-/// To model this, we define an abstract type of references to cache entries
-/// The type is indexed by the cache in which the entries reside
-val entry_ref (cache: t v) : Type
-(* Internally, entry_ref can be implemented as a pointer to a entry,
-    together with some specificational data, e.g., the indexed in the
-    cache to which it points. The liveness of an entry_ref is
-    determined by the liveness of the cache itself--so long as cache
-    is live, then all its entry_refs are usable *)
+/// We go for something simpler and assume clients of this module will keep
+/// track of an index, rather than manipulate raw values (this would greatly
+/// complicate the framing lemmas).
 
-/// A ghost deref of an entry_ref, for spec. TODO: consistent naming, e.g. entry_v?
-val entry_ref_value #cache(e:entry_ref cache)  (m:mem{cache_invariant cache mem}) : GTot entry
+/// Note that this returns a value via a dereference.
+val get_entry (#tr: VerifierTraits.t) (cache: t tr) (idx: vcache_idx { idx `FStar.UInt16.lt` tr.VerifierTraits.cache_size }):
+  Stack entry
+    (requires fun h0 ->
+      invariant h0 cache)
+    (requires fun h0 e h1 ->
+      e == Seq.index (entries h0 cache) (UInt16.v idx) /\
+      h0 == h1)
 
-/// The underlying index of an entry, ghostly
-val idx_of_entry (e:entry_ref cache) : GTot vcache_idx
-
-/// A lemma that ties together idx_of_entry, entry_ref_value and entries. Note
-/// that we have a mix of styles: the relationship between cache and e is
-/// expressed via an index, while the relationship between e and index is
-/// expressed via a predicate. TODO: figure out if there's a need to change this.
-val entry_ref_is_seq_index #cache (e: entry_ref cache) h idx: Lemma
-  (requires (idx_of_entry e == idx))
-  (ensures (
-    entry_ref_value e h == Seq.index (entries h cache) idx))
-
-/// We could then provide an API to gen an entry. JP: using m0 == m1 (no need to
-/// frame the invariant, no need to perform modifies-reasoning).
-val get_entry (v:Type) [| verifier_traits v |] (cache:t v) (idx:vcache_idx {idx < cacheSize})
-  : ST (entry_ref cache)
-       (requires fun m0 -> cache_invariant cache m0)
-       (requires fun m0 e m1 ->
-         idx_of_entry e == idx /\
-         m0 == m1)
+val set_entry (#tr: VerifierTraits.t) (cache: t tr)
+  (idx: vcache_idx { idx `FStar.UInt16.lt` tr.VerifierTraits.cache_size })
+  (entry: entry):
+  Stack unit
+    (requires fun h0 ->
+      invariant h0 cache)
+    (requires fun h0 _ h1 ->
+      invariant h1 cache /\
+      B.modifies (footprint cache) h0 h1 /\
+      entries h1 cache == Seq.upd (entries h0 cache) (UInt16.v idx) entry)
